src/Bedrock/Standalone/StandaloneHaskellMain.v
@@ -29,6 +29,11 @@ Module Bedrock2First.
       := main_gen ForExtraction.SaturatedSolinas.PipelineMain.
   End SaturatedSolinas.
 
+  Module BitcoinMultiplication.
+    Definition main : IO_unit
+      := main_gen ForExtraction.BitcoinMultiplication.PipelineMain.
+  End BitcoinMultiplication.
+
   Module BaseConversion.
     Definition main : IO_unit
       := main_gen ForExtraction.BaseConversion.PipelineMain.
@@ -57,6 +62,11 @@ Module Bedrock2Later.
     Definition main : IO_unit
       := main_gen ForExtraction.SaturatedSolinas.PipelineMain.
   End SaturatedSolinas.
+
+  Module BitcoinMultiplication.
+    Definition main : IO_unit
+      := main_gen ForExtraction.BitcoinMultiplication.PipelineMain.
+  End BitcoinMultiplication.
 
   Module BaseConversion.
     Definition main : IO_unit
