src/BitcoinMultiplication/CompilationOfOriginalAlgorithm.v
@@ -120,3 +120,4 @@ Time Redirect "log" Compute
                (None, (None, tt))
                None
    : Pipeline.ErrorT _).
+
